language/move-prover/src/prelude.bpl
@@ -18,14 +18,14 @@
 // Debug tracking is used to inject information used for model analysis. The generated code emits statements
 // like this:
 //
-//     assume $DebugTrackLocal(file_id, byte_index, var_idx, value);
+//     assume $DebugTrackLocal(file_id, byte_index, var_idx, $Value);
 //
 // While those tracking assumptions are trivially true for the provers logic, the solver (at least Z3)
 // will construct a function mapping which appears in the model, e.g.:
 //
 //     $DebugTrackLocal -> {
-//         1 440 0 (Vector (ValueArray |T@[Int]Value!val!0| 0)) -> true
-//         1 533 1 (Integer 1) -> true
+//         1 440 0 (Vector (ValueArray |T@[Int]$Value!val!0| 0)) -> true
+//         1 533 1 ($Integer 1) -> true
 //         ...
 //         else -> true
 //     }
@@ -35,7 +35,7 @@
 
 // Tracks debug information for a parameter, local or a return parameter. Return parameter indices start at
 // the overall number of locals (including parameters).
-function $DebugTrackLocal(file_id: int, byte_index:  int, var_idx: int, value: Value) : bool {
+function $DebugTrackLocal(file_id: int, byte_index:  int, var_idx: int, $Value: $Value) : bool {
   true
 }
 
@@ -44,162 +44,162 @@ function $DebugTrackAbort(file_id: int, byte_index: int) : bool {
   true
 }
 
-// Tracks the value of a specification (sub-)expression.
-function $DebugTrackExp(module_id: int, node_id: int, value: Value) : Value { value }
+// Tracks the $Value of a specification (sub-)expression.
+function $DebugTrackExp(module_id: int, node_id: int, $Value: $Value) : $Value { $Value }
 
 
 // Path type
 // ---------
 
-type {:datatype} Path;
-function {:constructor} Path(p: [int]int, size: int): Path;
-const EmptyPath: Path;
-axiom size#Path(EmptyPath) == 0;
+type {:datatype} $Path;
+function {:constructor} $Path(p: [int]int, size: int): $Path;
+const $EmptyPath: $Path;
+axiom size#$Path($EmptyPath) == 0;
 
-function {:inline} path_index_at(p: Path, i: int): int {
-    p#Path(p)[i]
+function {:inline} $path_index_at(p: $Path, i: int): int {
+    p#$Path(p)[i]
 }
 
 // Type Values
 // -----------
 
-type TypeName;
-type FieldName = int;
-type LocalName;
-type {:datatype} TypeValue;
-function {:constructor} BooleanType() : TypeValue;
-function {:constructor} IntegerType() : TypeValue;
-function {:constructor} AddressType() : TypeValue;
-function {:constructor} StrType() : TypeValue;
-function {:constructor} VectorType(t: TypeValue) : TypeValue;
-function {:constructor} StructType(name: TypeName, ps: TypeValueArray, ts: TypeValueArray) : TypeValue;
-function {:constructor} $TypeType(): TypeValue;
-function {:constructor} ErrorType() : TypeValue;
+type $TypeName;
+type $FieldName = int;
+type $LocalName;
+type {:datatype} $TypeValue;
+function {:constructor} $BooleanType() : $TypeValue;
+function {:constructor} $IntegerType() : $TypeValue;
+function {:constructor} $AddressType() : $TypeValue;
+function {:constructor} $StrType() : $TypeValue;
+function {:constructor} $VectorType(t: $TypeValue) : $TypeValue;
+function {:constructor} $StructType(name: $TypeName, ps: $TypeValueArray, ts: $TypeValueArray) : $TypeValue;
+function {:constructor} $TypeType(): $TypeValue;
+function {:constructor} $ErrorType() : $TypeValue;
 
-function {:inline} DefaultTypeValue() : TypeValue { ErrorType() }
-function {:builtin "MapConst"} MapConstTypeValue(tv: TypeValue): [int]TypeValue;
+function {:inline} $DefaultTypeValue() : $TypeValue { $ErrorType() }
+function {:builtin "MapConst"} $MapConstTypeValue(tv: $TypeValue): [int]$TypeValue;
 
-type {:datatype} TypeValueArray;
-function {:constructor} TypeValueArray(v: [int]TypeValue, l: int): TypeValueArray;
-const EmptyTypeValueArray: TypeValueArray;
-axiom l#TypeValueArray(EmptyTypeValueArray) == 0;
-axiom v#TypeValueArray(EmptyTypeValueArray) == MapConstTypeValue(DefaultTypeValue());
+type {:datatype} $TypeValueArray;
+function {:constructor} $TypeValueArray(v: [int]$TypeValue, l: int): $TypeValueArray;
+const $EmptyTypeValueArray: $TypeValueArray;
+axiom l#$TypeValueArray($EmptyTypeValueArray) == 0;
+axiom v#$TypeValueArray($EmptyTypeValueArray) == $MapConstTypeValue($DefaultTypeValue());
 
 
 // Values
 // ------
 
-type {:datatype} Value;
+type {:datatype} $Value;
 
-const MAX_U8: int;
-axiom MAX_U8 == 255;
-const MAX_U64: int;
-axiom MAX_U64 == 18446744073709551615;
-const MAX_U128: int;
-axiom MAX_U128 == 340282366920938463463374607431768211455;
+const $MAX_U8: int;
+axiom $MAX_U8 == 255;
+const $MAX_U64: int;
+axiom $MAX_U64 == 18446744073709551615;
+const $MAX_U128: int;
+axiom $MAX_U128 == 340282366920938463463374607431768211455;
 
-function {:constructor} Boolean(b: bool): Value;
-function {:constructor} Integer(i: int): Value;
-function {:constructor} Address(a: int): Value;
-function {:constructor} Vector(v: ValueArray): Value; // used to both represent move Struct and Vector
-function {:constructor} $Range(lb: Value, ub: Value): Value;
-function {:constructor} $Type(t: TypeValue): Value;
-function {:constructor} Error(): Value;
+function {:constructor} $Boolean(b: bool): $Value;
+function {:constructor} $Integer(i: int): $Value;
+function {:constructor} $Address(a: int): $Value;
+function {:constructor} $Vector(v: $ValueArray): $Value; // used to both represent move Struct and Vector
+function {:constructor} $Range(lb: $Value, ub: $Value): $Value;
+function {:constructor} $Type(t: $TypeValue): $Value;
+function {:constructor} $Error(): $Value;
 
-function {:inline} DefaultValue(): Value { Error() }
-function {:builtin "MapConst"} MapConstValue(v: Value): [int]Value;
+function {:inline} $DefaultValue(): $Value { $Error() }
+function {:builtin "MapConst"} $MapConstValue(v: $Value): [int]$Value;
 
-function {:inline} $IsValidU8(v: Value): bool {
-  is#Integer(v) && i#Integer(v) >= 0 && i#Integer(v) <= MAX_U8
+function {:inline} $IsValidU8(v: $Value): bool {
+  is#$Integer(v) && i#$Integer(v) >= 0 && i#$Integer(v) <= $MAX_U8
 }
 
-function {:inline} $IsValidU8Vector(vec: Value): bool {
+function {:inline} $IsValidU8Vector(vec: $Value): bool {
   $Vector_is_well_formed(vec)
   && (forall i: int :: {$vmap(vec)[i]} 0 <= i && i < $vlen(vec) ==> $IsValidU8($vmap(vec)[i]))
 }
 
-function {:inline} $IsValidU64(v: Value): bool {
-  is#Integer(v) && i#Integer(v) >= 0 && i#Integer(v) <= MAX_U64
+function {:inline} $IsValidU64(v: $Value): bool {
+  is#$Integer(v) && i#$Integer(v) >= 0 && i#$Integer(v) <= $MAX_U64
 }
 
-function {:inline} $IsValidU128(v: Value): bool {
-  is#Integer(v) && i#Integer(v) >= 0 && i#Integer(v) <= MAX_U128
+function {:inline} $IsValidU128(v: $Value): bool {
+  is#$Integer(v) && i#$Integer(v) >= 0 && i#$Integer(v) <= $MAX_U128
 }
 
-function {:inline} $IsValidNum(v: Value): bool {
-  is#Integer(v)
+function {:inline} $IsValidNum(v: $Value): bool {
+  is#$Integer(v)
 }
 
 
 // Value Array
 // -----------
 
-type {:datatype} ValueArray;
+type {:datatype} $ValueArray;
 
-function {:constructor} ValueArray(v: [int]Value, l: int): ValueArray;
-const EmptyValueArray: ValueArray;
+function {:constructor} $ValueArray(v: [int]$Value, l: int): $ValueArray;
+const $EmptyValueArray: $ValueArray;
 
-axiom l#ValueArray(EmptyValueArray) == 0;
-axiom v#ValueArray(EmptyValueArray) == MapConstValue(Error());
+axiom l#$ValueArray($EmptyValueArray) == 0;
+axiom v#$ValueArray($EmptyValueArray) == $MapConstValue($Error());
 
-function {{backend.func_inline}} RemoveValueArray(a: ValueArray): ValueArray {
+function {{backend.func_inline}} $RemoveValueArray(a: $ValueArray): $ValueArray {
     (
-        var l := l#ValueArray(a) - 1;
-        ValueArray(
+        var l := l#$ValueArray(a) - 1;
+        $ValueArray(
             (lambda i: int ::
-                if i >= 0 && i < l then v#ValueArray(a)[i] else DefaultValue()),
+                if i >= 0 && i < l then v#$ValueArray(a)[i] else $DefaultValue()),
             l
         )
     )
 }
-function {{backend.func_inline}} RemoveIndexValueArray(a: ValueArray, i: int): ValueArray {
+function {{backend.func_inline}} $RemoveIndexValueArray(a: $ValueArray, i: int): $ValueArray {
     (
-        var l := l#ValueArray(a) - 1;
-        ValueArray(
+        var l := l#$ValueArray(a) - 1;
+        $ValueArray(
             (lambda j: int ::
                 if j >= 0 && j < l then
-                    if j < i then v#ValueArray(a)[j] else v#ValueArray(a)[j+1]
-                else DefaultValue()),
+                    if j < i then v#$ValueArray(a)[j] else v#$ValueArray(a)[j+1]
+                else $DefaultValue()),
             l
         )
     )
 }
-function {{backend.func_inline}} ConcatValueArray(a1: ValueArray, a2: ValueArray): ValueArray {
+function {{backend.func_inline}} $ConcatValueArray(a1: $ValueArray, a2: $ValueArray): $ValueArray {
     (
-        var l1, l2 := l#ValueArray(a1), l#ValueArray(a2);
-        ValueArray(
+        var l1, l2 := l#$ValueArray(a1), l#$ValueArray(a2);
+        $ValueArray(
             (lambda i: int ::
                 if i >= 0 && i < l1 + l2 then
-                    if i < l1 then v#ValueArray(a1)[i] else v#ValueArray(a2)[i - l1]
+                    if i < l1 then v#$ValueArray(a1)[i] else v#$ValueArray(a2)[i - l1]
                 else
-                    DefaultValue()),
+                    $DefaultValue()),
             l1 + l2)
     )
 }
-function {{backend.func_inline}} ReverseValueArray(a: ValueArray): ValueArray {
+function {{backend.func_inline}} $ReverseValueArray(a: $ValueArray): $ValueArray {
     (
-        var l := l#ValueArray(a);
-        ValueArray(
-            (lambda i: int :: if 0 <= i && i < l then v#ValueArray(a)[l - i - 1] else DefaultValue()),
+        var l := l#$ValueArray(a);
+        $ValueArray(
+            (lambda i: int :: if 0 <= i && i < l then v#$ValueArray(a)[l - i - 1] else $DefaultValue()),
             l
         )
     )
 }
-function {{backend.func_inline}} SliceValueArray(a: ValueArray, i: int, j: int): ValueArray { // return the sliced vector of a for the range [i, j)
-    ValueArray((lambda k:int :: if 0 <= k && k < j-i then v#ValueArray(a)[i+k] else DefaultValue()), (if j-i < 0 then 0 else j-i))
+function {{backend.func_inline}} $SliceValueArray(a: $ValueArray, i: int, j: int): $ValueArray { // return the sliced vector of a for the range [i, j)
+    $ValueArray((lambda k:int :: if 0 <= k && k < j-i then v#$ValueArray(a)[i+k] else $DefaultValue()), (if j-i < 0 then 0 else j-i))
 }
-function {{backend.func_inline}} ExtendValueArray(a: ValueArray, elem: Value): ValueArray {
-    (var len := l#ValueArray(a);
-     ValueArray(v#ValueArray(a)[len := elem], len + 1))
+function {{backend.func_inline}} $ExtendValueArray(a: $ValueArray, elem: $Value): $ValueArray {
+    (var len := l#$ValueArray(a);
+     $ValueArray(v#$ValueArray(a)[len := elem], len + 1))
 }
-function {{backend.func_inline}} UpdateValueArray(a: ValueArray, i: int, elem: Value): ValueArray {
-    ValueArray(v#ValueArray(a)[i := elem], l#ValueArray(a))
+function {{backend.func_inline}} $UpdateValueArray(a: $ValueArray, i: int, elem: $Value): $ValueArray {
+    $ValueArray(v#$ValueArray(a)[i := elem], l#$ValueArray(a))
 }
-function {{backend.func_inline}} SwapValueArray(a: ValueArray, i: int, j: int): ValueArray {
-    ValueArray(v#ValueArray(a)[i := v#ValueArray(a)[j]][j := v#ValueArray(a)[i]], l#ValueArray(a))
+function {{backend.func_inline}} $SwapValueArray(a: $ValueArray, i: int, j: int): $ValueArray {
+    $ValueArray(v#$ValueArray(a)[i := v#$ValueArray(a)[j]][j := v#$ValueArray(a)[i]], l#$ValueArray(a))
 }
-function {:inline} IsEmpty(a: ValueArray): bool {
-    l#ValueArray(a) == 0
+function {:inline} $IsEmpty(a: $ValueArray): bool {
+    l#$ValueArray(a) == 0
 }
 
 // Stratified Functions on Values
@@ -209,14 +209,14 @@ function {:inline} IsEmpty(a: ValueArray): bool {
 //   prefer to handcode this so its easier to evolve the model independent of the
 //   translator.
 
-const StratificationDepth: int;
-axiom StratificationDepth == {{backend.stratification_depth}};
+const $StratificationDepth: int;
+axiom $StratificationDepth == {{backend.stratification_depth}};
 
 {{#if backend.native_equality}}
 
 // Map IsEqual to native Boogie equality. This only works with extensional arrays as provided
 // by the array theory.
-function {:inline} IsEqual(v1: Value, v2: Value): bool {
+function {:inline} $IsEqual(v1: $Value, v2: $Value): bool {
     v1 == v2
 }
 
@@ -224,21 +224,21 @@ function {:inline} IsEqual(v1: Value, v2: Value): bool {
 
 // Generate a stratified version of IsEqual for depth of {{backend.stratification_depth}}.
 {{#stratified}}
-function {{backend.aggressive_backend.func_inline}} IsEqual_{{@this_suffix}}(v1: Value, v2: Value): bool {
+function {{backend.aggressive_backend.func_inline}} $IsEqual_{{@this_suffix}}(v1: $Value, v2: $Value): bool {
     (v1 == v2) ||
-    (is#Vector(v1) &&
-     is#Vector(v2) &&
+    (is#$Vector(v1) &&
+     is#$Vector(v2) &&
      $vlen(v1) == $vlen(v2) &&
-     (forall i: int :: 0 <= i && i < $vlen(v1) ==> IsEqual_{{@next_suffix}}($vmap(v1)[i], $vmap(v2)[i])))
+     (forall i: int :: 0 <= i && i < $vlen(v1) ==> $IsEqual_{{@next_suffix}}($vmap(v1)[i], $vmap(v2)[i])))
 }
 {{else}}
-function {:inline} IsEqual_{{@this_suffix}}(v1: Value, v2: Value): bool {
+function {:inline} $IsEqual_{{@this_suffix}}(v1: $Value, v2: $Value): bool {
     v1 == v2
 }
 {{/stratified}}
 
-function {:inline} IsEqual(v1: Value, v2: Value): bool {
-    IsEqual_stratified(v1, v2)
+function {:inline} $IsEqual(v1: $Value, v2: $Value): bool {
+    $IsEqual_stratified(v1, v2)
 }
 
 {{/if}}
@@ -246,183 +246,183 @@ function {:inline} IsEqual(v1: Value, v2: Value): bool {
 // Generate stratified ReadValue for the depth of {{backend.stratification_depth}}.
 
 {{#stratified}}
-function {{backend.aggressive_backend.func_inline}} $ReadValue_{{@this_suffix}}(p: Path, v: Value) : Value {
-    if ({{@this_level}} == size#Path(p)) then
+function {{backend.aggressive_backend.func_inline}} $ReadValue_{{@this_suffix}}(p: $Path, v: $Value) : $Value {
+    if ({{@this_level}} == size#$Path(p)) then
         v
     else
-        $ReadValue_{{@next_suffix}}(p, $vmap(v)[path_index_at(p, {{@this_level}})])
+        $ReadValue_{{@next_suffix}}(p, $vmap(v)[$path_index_at(p, {{@this_level}})])
 }
 {{else}}
-function {:inline} $ReadValue_{{@this_suffix}}(p: Path, v: Value): Value {
+function {:inline} $ReadValue_{{@this_suffix}}(p: $Path, v: $Value): $Value {
     v
 }
 {{/stratified}}
 
-function {:inline} $ReadValue(p: Path, v: Value): Value {
+function {:inline} $ReadValue(p: $Path, v: $Value): $Value {
     $ReadValue_stratified(p, v)
 }
 
 // Generate stratified $UpdateValue for the depth of {{backend.stratification_depth}}.
 
 {{#stratified}}
-function {{backend.aggressive_backend.func_inline}} $UpdateValue_{{@this_suffix}}(p: Path, offset: int, v: Value, new_v: Value): Value {
+function {{backend.aggressive_backend.func_inline}} $UpdateValue_{{@this_suffix}}(p: $Path, offset: int, v: $Value, new_v: $Value): $Value {
     (var poffset := offset + {{@this_level}};
-    if (poffset == size#Path(p)) then
+    if (poffset == size#$Path(p)) then
         new_v
     else
-        $update_vector(v, path_index_at(p, poffset),
-                       $UpdateValue_{{@next_suffix}}(p, offset, $vmap(v)[path_index_at(p, poffset)], new_v)))
+        $update_vector(v, $path_index_at(p, poffset),
+                       $UpdateValue_{{@next_suffix}}(p, offset, $vmap(v)[$path_index_at(p, poffset)], new_v)))
 }
 {{else}}
-function {:inline} $UpdateValue_{{@this_suffix}}(p: Path, offset: int, v: Value, new_v: Value): Value {
+function {:inline} $UpdateValue_{{@this_suffix}}(p: $Path, offset: int, v: $Value, new_v: $Value): $Value {
     new_v
 }
 {{/stratified}}
 
-function {:inline} $UpdateValue(p: Path, offset: int, v: Value, new_v: Value): Value {
+function {:inline} $UpdateValue(p: $Path, offset: int, v: $Value, new_v: $Value): $Value {
     $UpdateValue_stratified(p, offset, v, new_v)
 }
 
 // Generate stratified $IsPathPrefix for the depth of {{backend.stratification_depth}}.
 
 {{#stratified}}
-function {{backend.aggressive_backend.func_inline}} $IsPathPrefix_{{@this_suffix}}(p1: Path, p2: Path): bool {
-    if ({{@this_level}} == size#Path(p1)) then
+function {{backend.aggressive_backend.func_inline}} $IsPathPrefix_{{@this_suffix}}(p1: $Path, p2: $Path): bool {
+    if ({{@this_level}} == size#$Path(p1)) then
         true
-    else if (p#Path(p1)[{{@this_level}}] == p#Path(p2)[{{@this_level}}]) then
+    else if (p#$Path(p1)[{{@this_level}}] == p#$Path(p2)[{{@this_level}}]) then
         $IsPathPrefix_{{@next_suffix}}(p1, p2)
     else
         false
 }
 {{else}}
-function {:inline} $IsPathPrefix_{{@this_suffix}}(p1: Path, p2: Path): bool {
+function {:inline} $IsPathPrefix_{{@this_suffix}}(p1: $Path, p2: $Path): bool {
     true
 }
 {{/stratified}}
 
-function {:inline} $IsPathPrefix(p1: Path, p2: Path): bool {
+function {:inline} $IsPathPrefix(p1: $Path, p2: $Path): bool {
     $IsPathPrefix_stratified(p1, p2)
 }
 
 // Generate stratified $ConcatPath for the depth of {{backend.stratification_depth}}.
 
 {{#stratified}}
-function {{backend.aggressive_backend.func_inline}} $ConcatPath_{{@this_suffix}}(p1: Path, p2: Path): Path {
-    if ({{@this_level}} == size#Path(p2)) then
+function {{backend.aggressive_backend.func_inline}} $ConcatPath_{{@this_suffix}}(p1: $Path, p2: $Path): $Path {
+    if ({{@this_level}} == size#$Path(p2)) then
         p1
     else
-        $ConcatPath_{{@next_suffix}}(Path(p#Path(p1)[size#Path(p1) := p#Path(p2)[{{@this_level}}]], size#Path(p1) + 1), p2)
+        $ConcatPath_{{@next_suffix}}($Path(p#$Path(p1)[size#$Path(p1) := p#$Path(p2)[{{@this_level}}]], size#$Path(p1) + 1), p2)
 }
 {{else}}
-function {:inline} $ConcatPath_{{@this_suffix}}(p1: Path, p2: Path): Path {
+function {:inline} $ConcatPath_{{@this_suffix}}(p1: $Path, p2: $Path): $Path {
     p1
 }
 {{/stratified}}
 
-function {:inline} $ConcatPath(p1: Path, p2: Path): Path {
+function {:inline} $ConcatPath(p1: $Path, p2: $Path): $Path {
     $ConcatPath_stratified(p1, p2)
 }
 
-// Vector related functions on values
+// Vector related functions on Values
 // ----------------------------------
 
-function {:inline} $vmap(v: Value): [int]Value {
-    v#ValueArray(v#Vector(v))
+function {:inline} $vmap(v: $Value): [int]$Value {
+    v#$ValueArray(v#$Vector(v))
 }
-function {:inline} $vlen(v: Value): int {
-    l#ValueArray(v#Vector(v))
+function {:inline} $vlen(v: $Value): int {
+    l#$ValueArray(v#$Vector(v))
 }
 
 // All invalid elements of array are DefaultValue. This is useful in specialized
 // cases
-function {:inline} IsNormalizedMap(va: [int]Value, len: int): bool {
-    (forall i: int :: i < 0 || i >= len ==> va[i] == DefaultValue())
+function {:inline} $IsNormalizedMap(va: [int]$Value, len: int): bool {
+    (forall i: int :: i < 0 || i >= len ==> va[i] == $DefaultValue())
 }
 
 // Check that all invalid elements of vector are DefaultValue
-function {:inline} $is_normalized_vector(v: Value): bool {
-    IsNormalizedMap($vmap(v), $vlen(v))
+function {:inline} $is_normalized_vector(v: $Value): bool {
+    $IsNormalizedMap($vmap(v), $vlen(v))
 }
 
 // Sometimes, we need the length as a Value, not an int.
-function {:inline} $vlen_value(v: Value): Value {
-    Integer($vlen(v))
+function {:inline} $vlen_value(v: $Value): $Value {
+    $Integer($vlen(v))
 }
-function {:inline} $mk_vector(): Value {
-    Vector(EmptyValueArray)
+function {:inline} $mk_vector(): $Value {
+    $Vector($EmptyValueArray)
 }
-function {:inline} $push_back_vector(v: Value, elem: Value): Value {
-    Vector(ExtendValueArray(v#Vector(v), elem))
+function {:inline} $push_back_vector(v: $Value, elem: $Value): $Value {
+    $Vector($ExtendValueArray(v#$Vector(v), elem))
 }
-function {:inline} $pop_back_vector(v: Value): Value {
-    Vector(RemoveValueArray(v#Vector(v)))
+function {:inline} $pop_back_vector(v: $Value): $Value {
+    $Vector($RemoveValueArray(v#$Vector(v)))
 }
-function {:inline} $append_vector(v1: Value, v2: Value): Value {
-    Vector(ConcatValueArray(v#Vector(v1), v#Vector(v2)))
+function {:inline} $append_vector(v1: $Value, v2: $Value): $Value {
+    $Vector($ConcatValueArray(v#$Vector(v1), v#$Vector(v2)))
 }
-function {:inline} $reverse_vector(v: Value): Value {
-    Vector(ReverseValueArray(v#Vector(v)))
+function {:inline} $reverse_vector(v: $Value): $Value {
+    $Vector($ReverseValueArray(v#$Vector(v)))
 }
-function {:inline} $update_vector(v: Value, i: int, elem: Value): Value {
-    Vector(UpdateValueArray(v#Vector(v), i, elem))
+function {:inline} $update_vector(v: $Value, i: int, elem: $Value): $Value {
+    $Vector($UpdateValueArray(v#$Vector(v), i, elem))
 }
 // $update_vector_by_value requires index to be a Value, not int.
-function {:inline} $update_vector_by_value(v: Value, i: Value, elem: Value): Value {
-    Vector(UpdateValueArray(v#Vector(v), i#Integer(i), elem))
+function {:inline} $update_vector_by_value(v: $Value, i: $Value, elem: $Value): $Value {
+    $Vector($UpdateValueArray(v#$Vector(v), i#$Integer(i), elem))
 }
-function {:inline} $select_vector(v: Value, i: int) : Value {
+function {:inline} $select_vector(v: $Value, i: int) : $Value {
     $vmap(v)[i]
 }
 // $select_vector_by_value requires index to be a Value, not int.
-function {:inline} $select_vector_by_value(v: Value, i: Value) : Value {
-    $vmap(v)[i#Integer(i)]
+function {:inline} $select_vector_by_value(v: $Value, i: $Value) : $Value {
+    $vmap(v)[i#$Integer(i)]
 }
-function {:inline} $swap_vector(v: Value, i: int, j: int): Value {
-    Vector(SwapValueArray(v#Vector(v), i, j))
+function {:inline} $swap_vector(v: $Value, i: int, j: int): $Value {
+    $Vector($SwapValueArray(v#$Vector(v), i, j))
 }
-function {:inline} $slice_vector(v: Value, r: Value) : Value {
-    Vector(SliceValueArray(v#Vector(v), i#Integer(lb#$Range(r)), i#Integer(ub#$Range(r))))
+function {:inline} $slice_vector(v: $Value, r: $Value) : $Value {
+    $Vector($SliceValueArray(v#$Vector(v), i#$Integer(lb#$Range(r)), i#$Integer(ub#$Range(r))))
 }
-function {:inline} $InVectorRange(v: Value, i: int): bool {
+function {:inline} $InVectorRange(v: $Value, i: int): bool {
     i >= 0 && i < $vlen(v)
 }
-function {:inline} $remove_vector(v: Value, i:int): Value {
-    Vector(RemoveIndexValueArray(v#Vector(v), i))
+function {:inline} $remove_vector(v: $Value, i:int): $Value {
+    $Vector($RemoveIndexValueArray(v#$Vector(v), i))
 }
-function {:inline} $contains_vector(v: Value, e: Value): bool {
-    (exists i:int :: 0<=i && i<$vlen(v) && IsEqual($vmap(v)[i], e))
+function {:inline} $contains_vector(v: $Value, e: $Value): bool {
+    (exists i:int :: 0<=i && i<$vlen(v) && $IsEqual($vmap(v)[i], e))
 }
 
-function {:inline} $InRange(r: Value, i: int): bool {
-   i#Integer(lb#$Range(r)) <= i && i < i#Integer(ub#$Range(r))
+function {:inline} $InRange(r: $Value, i: int): bool {
+   i#$Integer(lb#$Range(r)) <= i && i < i#$Integer(ub#$Range(r))
 }
 
 
 // ============================================================================================
 // Memory
 
-type {:datatype} Location;
-function {:constructor} Global(t: TypeValue, a: int): Location;
-function {:constructor} Local(i: int): Location;
-function {:constructor} Param(i: int): Location;
+type {:datatype} $Location;
+function {:constructor} $Global(t: $TypeValue, a: int): $Location;
+function {:constructor} $Local(i: int): $Location;
+function {:constructor} $Param(i: int): $Location;
 
-type {:datatype} Reference;
-function {:constructor} Reference(l: Location, p: Path, v: Value): Reference;
-const DefaultReference: Reference;
+type {:datatype} $Reference;
+function {:constructor} $Reference(l: $Location, p: $Path, v: $Value): $Reference;
+const $DefaultReference: $Reference;
 
-type {:datatype} Memory;
-function {:constructor} Memory(domain: [Location]bool, contents: [Location]Value): Memory;
+type {:datatype} $Memory;
+function {:constructor} $Memory(domain: [$Location]bool, contents: [$Location]$Value): $Memory;
 
-function $Memory__is_well_formed(m: Memory): bool;
+function $Memory__is_well_formed(m: $Memory): bool;
 
-function {:builtin "MapConst"} ConstMemoryDomain(v: bool): [Location]bool;
-function {:builtin "MapConst"} ConstMemoryContent(v: Value): [Location]Value;
+function {:builtin "MapConst"} $ConstMemoryDomain(v: bool): [$Location]bool;
+function {:builtin "MapConst"} $ConstMemoryContent(v: $Value): [$Location]$Value;
 
-const EmptyMemory: Memory;
-axiom domain#Memory(EmptyMemory) == ConstMemoryDomain(false);
-axiom contents#Memory(EmptyMemory) == ConstMemoryContent(DefaultValue());
+const $EmptyMemory: $Memory;
+axiom domain#$Memory($EmptyMemory) == $ConstMemoryDomain(false);
+axiom contents#$Memory($EmptyMemory) == $ConstMemoryContent($DefaultValue());
 
-var $m: Memory;
+var $m: $Memory;
 var $abort_flag: bool;
 
 procedure {:inline 1} $InitVerification() {
@@ -436,401 +436,401 @@ procedure {:inline 1} $InitVerification() {
 // TODO: unify some of this with instruction procedures to avoid duplication
 
 // Tests whether resource exists.
-function {:inline} $ResourceExistsRaw(m: Memory, resource: TypeValue, addr: int): bool {
-    domain#Memory(m)[Global(resource, addr)]
+function {:inline} $ResourceExistsRaw(m: $Memory, resource: $TypeValue, addr: int): bool {
+    domain#$Memory(m)[$Global(resource, addr)]
 }
-function {:inline} $ResourceExists(m: Memory, resource: TypeValue, address: Value): Value {
-    Boolean($ResourceExistsRaw(m, resource, a#Address(address)))
-}
-
-// Obtains value of given resource.
-function {:inline} $ResourceValue(m: Memory, resource: TypeValue, address: Value): Value {
-  contents#Memory(m)[Global(resource, a#Address(address))]
+function {:inline} $ResourceExists(m: $Memory, resource: $TypeValue, address: $Value): $Value {
+    $Boolean($ResourceExistsRaw(m, resource, a#$Address(address)))
 }
 
-// Applies a field selection to a value.
-function {:inline} $SelectField(val: Value, field: FieldName): Value {
+// Obtains Value of given resource.
+function {:inline} $ResourceValue(m: $Memory, resource: $TypeValue, address: $Value): $Value {
+  contents#$Memory(m)[$Global(resource, a#$Address(address))]
+}
+
+// Applies a field selection to a Value.
+function {:inline} $SelectField(val: $Value, field: $FieldName): $Value {
     $vmap(val)[field]
 }
 
 // Dereferences a reference.
-function {:inline} $Dereference(ref: Reference): Value {
-    v#Reference(ref)
+function {:inline} $Dereference(ref: $Reference): $Value {
+    v#$Reference(ref)
 }
 
 // Check whether sender account exists.
-function {:inline} $ExistsTxnSenderAccount(m: Memory, txn: Transaction): bool {
-   domain#Memory(m)[Global($LibraAccount_T_type_value(), sender#Transaction(txn))]
+function {:inline} $ExistsTxnSenderAccount(m: $Memory, txn: $Transaction): bool {
+   domain#$Memory(m)[$Global($LibraAccount_T_type_value(), sender#$Transaction(txn))]
 }
 
-function {:inline} $TxnSender(txn: Transaction): Value {
-    Address(sender#Transaction(txn))
+function {:inline} $TxnSender(txn: $Transaction): $Value {
+    $Address(sender#$Transaction(txn))
 }
 
-// Forward declaration of type value of LibraAccount. This is declared so we can define
+// Forward declaration of type Value of LibraAccount. This is declared so we can define
 // $ExistsTxnSenderAccount and $LibraAccount_save_account
-function $LibraAccount_T_type_value(): TypeValue;
+function $LibraAccount_T_type_value(): $TypeValue;
 
-function $LibraAccount_Balance_type_value(tv: TypeValue): TypeValue;
+function $LibraAccount_Balance_type_value(tv: $TypeValue): $TypeValue;
 
 // ============================================================================================
 // Instructions
 
-procedure {:inline 1} $Exists(address: Value, t: TypeValue) returns (dst: Value)
-{{backend.type_requires}} is#Address(address);
+procedure {:inline 1} $Exists(address: $Value, t: $TypeValue) returns (dst: $Value)
+{{backend.type_requires}} is#$Address(address);
 {
     dst := $ResourceExists($m, t, address);
 }
 
-procedure {:inline 1} $MoveToRaw(ta: TypeValue, a: int, v: Value)
+procedure {:inline 1} $MoveToRaw(ta: $TypeValue, a: int, v: $Value)
 {
-    var l: Location;
+    var l: $Location;
 
-    l := Global(ta, a);
+    l := $Global(ta, a);
     if ($ResourceExistsRaw($m, ta, a)) {
         $abort_flag := true;
         return;
     }
-    $m := Memory(domain#Memory($m)[l := true], contents#Memory($m)[l := v]);
+    $m := $Memory(domain#$Memory($m)[l := true], contents#$Memory($m)[l := v]);
 }
 
-procedure {:inline 1} $MoveTo(ta: TypeValue, v: Value, signer: Value)
+procedure {:inline 1} $MoveTo(ta: $TypeValue, v: $Value, signer: $Value)
 {
-    var addr: Value;
+    var addr: $Value;
 
     call addr := $Signer_borrow_address(signer);
-    call $MoveToRaw(ta, a#Address(addr), v);
+    call $MoveToRaw(ta, a#$Address(addr), v);
 }
 
-procedure {:inline 1} $MoveToSender(ta: TypeValue, v: Value)
+procedure {:inline 1} $MoveToSender(ta: $TypeValue, v: $Value)
 {
-    call $MoveToRaw(ta, sender#Transaction($txn), v);
+    call $MoveToRaw(ta, sender#$Transaction($txn), v);
 }
 
-procedure {:inline 1} $MoveFrom(address: Value, ta: TypeValue) returns (dst: Value)
-{{backend.type_requires}} is#Address(address);
+procedure {:inline 1} $MoveFrom(address: $Value, ta: $TypeValue) returns (dst: $Value)
+{{backend.type_requires}} is#$Address(address);
 {
     var a: int;
-    var l: Location;
-    a := a#Address(address);
-    l := Global(ta, a);
+    var l: $Location;
+    a := a#$Address(address);
+    l := $Global(ta, a);
     if (!$ResourceExistsRaw($m, ta, a)) {
         $abort_flag := true;
         return;
     }
-    dst := contents#Memory($m)[l];
-    $m := Memory(domain#Memory($m)[l := false], contents#Memory($m)[l := DefaultValue()]);
+    dst := contents#$Memory($m)[l];
+    $m := $Memory(domain#$Memory($m)[l := false], contents#$Memory($m)[l := $DefaultValue()]);
 }
 
-procedure {:inline 1} $BorrowGlobal(address: Value, ta: TypeValue) returns (dst: Reference)
-{{backend.type_requires}} is#Address(address);
+procedure {:inline 1} $BorrowGlobal(address: $Value, ta: $TypeValue) returns (dst: $Reference)
+{{backend.type_requires}} is#$Address(address);
 {
     var a: int;
-    var l: Location;
-    a := a#Address(address);
-    l := Global(ta, a);
+    var l: $Location;
+    a := a#$Address(address);
+    l := $Global(ta, a);
     if (!$ResourceExistsRaw($m, ta, a)) {
         $abort_flag := true;
         return;
     }
-    dst := Reference(l, EmptyPath, contents#Memory($m)[l]);
+    dst := $Reference(l, $EmptyPath, contents#$Memory($m)[l]);
 }
 
-procedure {:inline 1} $BorrowLoc(l: int, v: Value) returns (dst: Reference)
+procedure {:inline 1} $BorrowLoc(l: int, v: $Value) returns (dst: $Reference)
 {
-    dst := Reference(Local(l), EmptyPath, v);
+    dst := $Reference($Local(l), $EmptyPath, v);
 }
 
-procedure {:inline 1} $BorrowField(src: Reference, f: FieldName) returns (dst: Reference)
+procedure {:inline 1} $BorrowField(src: $Reference, f: $FieldName) returns (dst: $Reference)
 {
-    var p: Path;
+    var p: $Path;
     var size: int;
 
-    p := p#Reference(src);
-    size := size#Path(p);
-    p := Path(p#Path(p)[size := f], size+1);
-    dst := Reference(l#Reference(src), p, $vmap(v#Reference(src))[f]);
+    p := p#$Reference(src);
+    size := size#$Path(p);
+    p := $Path(p#$Path(p)[size := f], size+1);
+    dst := $Reference(l#$Reference(src), p, $vmap(v#$Reference(src))[f]);
 }
 
-procedure {:inline 1} $GetGlobal(address: Value, ta: TypeValue) returns (dst: Value)
-{{backend.type_requires}} is#Address(address);
+procedure {:inline 1} $GetGlobal(address: $Value, ta: $TypeValue) returns (dst: $Value)
+{{backend.type_requires}} is#$Address(address);
 {
-    var r: Reference;
+    var r: $Reference;
 
     call r := $BorrowGlobal(address, ta);
     call dst := $ReadRef(r);
 }
 
-procedure {:inline 1} $GetFieldFromReference(src: Reference, f: FieldName) returns (dst: Value)
+procedure {:inline 1} $GetFieldFromReference(src: $Reference, f: $FieldName) returns (dst: $Value)
 {
-    var r: Reference;
+    var r: $Reference;
 
     call r := $BorrowField(src, f);
     call dst := $ReadRef(r);
 }
 
-procedure {:inline 1} $GetFieldFromValue(src: Value, f: FieldName) returns (dst: Value)
+procedure {:inline 1} $GetFieldFromValue(src: $Value, f: $FieldName) returns (dst: $Value)
 {
     dst := $vmap(src)[f];
 }
 
-procedure {:inline 1} $WriteRef(to: Reference, new_v: Value) returns (to': Reference)
+procedure {:inline 1} $WriteRef(to: $Reference, new_v: $Value) returns (to': $Reference)
 {
-    to' := Reference(l#Reference(to), p#Reference(to), new_v);
+    to' := $Reference(l#$Reference(to), p#$Reference(to), new_v);
 }
 
-procedure {:inline 1} $ReadRef(from: Reference) returns (v: Value)
+procedure {:inline 1} $ReadRef(from: $Reference) returns (v: $Value)
 {
-    v := v#Reference(from);
+    v := v#$Reference(from);
 }
 
-procedure {:inline 1} $CopyOrMoveRef(local: Reference) returns (dst: Reference)
+procedure {:inline 1} $CopyOrMoveRef(local: $Reference) returns (dst: $Reference)
 {
     dst := local;
 }
 
-procedure {:inline 1} $CopyOrMoveValue(local: Value) returns (dst: Value)
+procedure {:inline 1} $CopyOrMoveValue(local: $Value) returns (dst: $Value)
 {
     dst := local;
 }
 
-procedure {:inline 1} WritebackToGlobal(src: Reference)
+procedure {:inline 1} $WritebackToGlobal(src: $Reference)
 {
-    var l: Location;
-    var v: Value;
+    var l: $Location;
+    var v: $Value;
 
-    l := l#Reference(src);
-    if (is#Global(l)) {
-        v := $UpdateValue(p#Reference(src), 0, contents#Memory($m)[l], v#Reference(src));
-        $m := Memory(domain#Memory($m), contents#Memory($m)[l := v]);
+    l := l#$Reference(src);
+    if (is#$Global(l)) {
+        v := $UpdateValue(p#$Reference(src), 0, contents#$Memory($m)[l], v#$Reference(src));
+        $m := $Memory(domain#$Memory($m), contents#$Memory($m)[l := v]);
     }
 }
 
-procedure {:inline 1} WritebackToValue(src: Reference, idx: int, vdst: Value) returns (vdst': Value)
+procedure {:inline 1} $WritebackToValue(src: $Reference, idx: int, vdst: $Value) returns (vdst': $Value)
 {
-    if (l#Reference(src) == Local(idx)) {
-        vdst' := $UpdateValue(p#Reference(src), 0, vdst, v#Reference(src));
+    if (l#$Reference(src) == $Local(idx)) {
+        vdst' := $UpdateValue(p#$Reference(src), 0, vdst, v#$Reference(src));
     } else {
         vdst' := vdst;
     }
 }
 
-procedure {:inline 1} WritebackToReference(src: Reference, dst: Reference) returns (dst': Reference)
+procedure {:inline 1} $WritebackToReference(src: $Reference, dst: $Reference) returns (dst': $Reference)
 {
-    var srcPath, dstPath: Path;
+    var srcPath, dstPath: $Path;
 
-    srcPath := p#Reference(src);
-    dstPath := p#Reference(dst);
-    if (l#Reference(dst) == l#Reference(src) && size#Path(dstPath) <= size#Path(srcPath) && $IsPathPrefix(dstPath, srcPath)) {
-        dst' := Reference(
-                    l#Reference(dst),
+    srcPath := p#$Reference(src);
+    dstPath := p#$Reference(dst);
+    if (l#$Reference(dst) == l#$Reference(src) && size#$Path(dstPath) <= size#$Path(srcPath) && $IsPathPrefix(dstPath, srcPath)) {
+        dst' := $Reference(
+                    l#$Reference(dst),
                     dstPath,
-                    $UpdateValue(srcPath, size#Path(dstPath), v#Reference(dst), v#Reference(src)));
+                    $UpdateValue(srcPath, size#$Path(dstPath), v#$Reference(dst), v#$Reference(src)));
     } else {
         dst' := dst;
     }
 }
 
-procedure {:inline 1} Splice1(idx1: int, src1:Reference, dst: Reference) returns (dst': Reference) {
-    assume l#Reference(dst) == Local(idx1);
-    dst' := Reference(l#Reference(dst), $ConcatPath(p#Reference(src1), p#Reference(dst)), v#Reference(dst));
+procedure {:inline 1} $Splice1(idx1: int, src1: $Reference, dst: $Reference) returns (dst': $Reference) {
+    assume l#$Reference(dst) == $Local(idx1);
+    dst' := $Reference(l#$Reference(dst), $ConcatPath(p#$Reference(src1), p#$Reference(dst)), v#$Reference(dst));
 }
 
-procedure {:inline 1} $CastU8(src: Value) returns (dst: Value)
-{{backend.type_requires}} is#Integer(src);
+procedure {:inline 1} $CastU8(src: $Value) returns (dst: $Value)
+{{backend.type_requires}} is#$Integer(src);
 {
-    if (i#Integer(src) > MAX_U8) {
+    if (i#$Integer(src) > $MAX_U8) {
         $abort_flag := true;
         return;
     }
     dst := src;
 }
 
-procedure {:inline 1} $CastU64(src: Value) returns (dst: Value)
-{{backend.type_requires}} is#Integer(src);
+procedure {:inline 1} $CastU64(src: $Value) returns (dst: $Value)
+{{backend.type_requires}} is#$Integer(src);
 {
-    if (i#Integer(src) > MAX_U64) {
+    if (i#$Integer(src) > $MAX_U64) {
         $abort_flag := true;
         return;
     }
     dst := src;
 }
 
-procedure {:inline 1} $CastU128(src: Value) returns (dst: Value)
-{{backend.type_requires}} is#Integer(src);
+procedure {:inline 1} $CastU128(src: $Value) returns (dst: $Value)
+{{backend.type_requires}} is#$Integer(src);
 {
-    if (i#Integer(src) > MAX_U128) {
+    if (i#$Integer(src) > $MAX_U128) {
         $abort_flag := true;
         return;
     }
     dst := src;
 }
 
-procedure {:inline 1} $AddU8(src1: Value, src2: Value) returns (dst: Value)
+procedure {:inline 1} $AddU8(src1: $Value, src2: $Value) returns (dst: $Value)
 {{backend.type_requires}} $IsValidU8(src1) && $IsValidU8(src2);
 {
-    if (i#Integer(src1) + i#Integer(src2) > MAX_U8) {
+    if (i#$Integer(src1) + i#$Integer(src2) > $MAX_U8) {
         $abort_flag := true;
         return;
     }
-    dst := Integer(i#Integer(src1) + i#Integer(src2));
+    dst := $Integer(i#$Integer(src1) + i#$Integer(src2));
 }
 
-procedure {:inline 1} $AddU64(src1: Value, src2: Value) returns (dst: Value)
+procedure {:inline 1} $AddU64(src1: $Value, src2: $Value) returns (dst: $Value)
 {{backend.type_requires}} $IsValidU64(src1) && $IsValidU64(src2);
 {
-    if (i#Integer(src1) + i#Integer(src2) > MAX_U64) {
+    if (i#$Integer(src1) + i#$Integer(src2) > $MAX_U64) {
         $abort_flag := true;
         return;
     }
-    dst := Integer(i#Integer(src1) + i#Integer(src2));
+    dst := $Integer(i#$Integer(src1) + i#$Integer(src2));
 }
 
-procedure {:inline 1} $AddU128(src1: Value, src2: Value) returns (dst: Value)
+procedure {:inline 1} $AddU128(src1: $Value, src2: $Value) returns (dst: $Value)
 {{backend.type_requires}} $IsValidU128(src1) && $IsValidU128(src2);
 {
-    if (i#Integer(src1) + i#Integer(src2) > MAX_U128) {
+    if (i#$Integer(src1) + i#$Integer(src2) > $MAX_U128) {
         $abort_flag := true;
         return;
     }
-    dst := Integer(i#Integer(src1) + i#Integer(src2));
+    dst := $Integer(i#$Integer(src1) + i#$Integer(src2));
 }
 
-procedure {:inline 1} $Sub(src1: Value, src2: Value) returns (dst: Value)
-{{backend.type_requires}} is#Integer(src1) && is#Integer(src2);
+procedure {:inline 1} $Sub(src1: $Value, src2: $Value) returns (dst: $Value)
+{{backend.type_requires}} is#$Integer(src1) && is#$Integer(src2);
 {
-    if (i#Integer(src1) < i#Integer(src2)) {
+    if (i#$Integer(src1) < i#$Integer(src2)) {
         $abort_flag := true;
         return;
     }
-    dst := Integer(i#Integer(src1) - i#Integer(src2));
+    dst := $Integer(i#$Integer(src1) - i#$Integer(src2));
 }
 
 // This deals only with narrow special cases. Src2 must be constant
 // 32 or 64, which is what we use now.  Obviously, it could be extended
-// to src2 == any integer value from 0..127.
+// to src2 == any integer Value from 0..127.
 // Left them out for brevity
-function power_of_2 (power:Value): int {
-    (var p := i#Integer(power);
+function $power_of_2(power: $Value): int {
+    (var p := i#$Integer(power);
      if p == 32 then 4294967296
      else if p == 64 then 18446744073709551616
-     // value is undefined, otherwise.
+     // Value is undefined, otherwise.
      else -1
      )
 }
 
-procedure {:inline 1} $Shl(src1: Value, src2: Value) returns (dst: Value)
-requires is#Integer(src1) && is#Integer(src2);
+procedure {:inline 1} $Shl(src1: $Value, src2: $Value) returns (dst: $Value)
+requires is#$Integer(src1) && is#$Integer(src2);
 {
     var po2: int;
-    po2 := power_of_2(src2);
+    po2 := $power_of_2(src2);
     assert po2 >= 1;   // po2 < 0 if src2 not 32 or 63
-    dst := Integer(i#Integer(src2) * po2);
+    dst := $Integer(i#$Integer(src2) * po2);
 }
 
-procedure {:inline 1} $Shr(src1: Value, src2: Value) returns (dst: Value)
-requires is#Integer(src1) && is#Integer(src2);
+procedure {:inline 1} $Shr(src1: $Value, src2: $Value) returns (dst: $Value)
+requires is#$Integer(src1) && is#$Integer(src2);
 {
     var po2: int;
-    po2 := power_of_2(src2);
+    po2 := $power_of_2(src2);
     assert po2 >= 1;   // po2 < 0 if src2 not 32 or 63
-    dst := Integer(i#Integer(src2) div po2);
+    dst := $Integer(i#$Integer(src2) div po2);
 }
 
-procedure {:inline 1} $MulU8(src1: Value, src2: Value) returns (dst: Value)
+procedure {:inline 1} $MulU8(src1: $Value, src2: $Value) returns (dst: $Value)
 {{backend.type_requires}} $IsValidU8(src1) && $IsValidU8(src2);
 {
-    if (i#Integer(src1) * i#Integer(src2) > MAX_U8) {
+    if (i#$Integer(src1) * i#$Integer(src2) > $MAX_U8) {
         $abort_flag := true;
         return;
     }
-    dst := Integer(i#Integer(src1) * i#Integer(src2));
+    dst := $Integer(i#$Integer(src1) * i#$Integer(src2));
 }
 
-procedure {:inline 1} $MulU64(src1: Value, src2: Value) returns (dst: Value)
+procedure {:inline 1} $MulU64(src1: $Value, src2: $Value) returns (dst: $Value)
 {{backend.type_requires}} $IsValidU64(src1) && $IsValidU64(src2);
 {
-    if (i#Integer(src1) * i#Integer(src2) > MAX_U64) {
+    if (i#$Integer(src1) * i#$Integer(src2) > $MAX_U64) {
         $abort_flag := true;
         return;
     }
-    dst := Integer(i#Integer(src1) * i#Integer(src2));
+    dst := $Integer(i#$Integer(src1) * i#$Integer(src2));
 }
 
-procedure {:inline 1} $MulU128(src1: Value, src2: Value) returns (dst: Value)
+procedure {:inline 1} $MulU128(src1: $Value, src2: $Value) returns (dst: $Value)
 {{backend.type_requires}} $IsValidU128(src1) && $IsValidU128(src2);
 {
-    if (i#Integer(src1) * i#Integer(src2) > MAX_U128) {
+    if (i#$Integer(src1) * i#$Integer(src2) > $MAX_U128) {
         $abort_flag := true;
         return;
     }
-    dst := Integer(i#Integer(src1) * i#Integer(src2));
+    dst := $Integer(i#$Integer(src1) * i#$Integer(src2));
 }
 
-procedure {:inline 1} $Div(src1: Value, src2: Value) returns (dst: Value)
-{{backend.type_requires}} is#Integer(src1) && is#Integer(src2);
+procedure {:inline 1} $Div(src1: $Value, src2: $Value) returns (dst: $Value)
+{{backend.type_requires}} is#$Integer(src1) && is#$Integer(src2);
 {
-    if (i#Integer(src2) == 0) {
+    if (i#$Integer(src2) == 0) {
         $abort_flag := true;
         return;
     }
-    dst := Integer(i#Integer(src1) div i#Integer(src2));
+    dst := $Integer(i#$Integer(src1) div i#$Integer(src2));
 }
 
-procedure {:inline 1} $Mod(src1: Value, src2: Value) returns (dst: Value)
-{{backend.type_requires}} is#Integer(src1) && is#Integer(src2);
+procedure {:inline 1} $Mod(src1: $Value, src2: $Value) returns (dst: $Value)
+{{backend.type_requires}} is#$Integer(src1) && is#$Integer(src2);
 {
-    if (i#Integer(src2) == 0) {
+    if (i#$Integer(src2) == 0) {
         $abort_flag := true;
         return;
     }
-    dst := Integer(i#Integer(src1) mod i#Integer(src2));
+    dst := $Integer(i#$Integer(src1) mod i#$Integer(src2));
 }
 
-procedure {:inline 1} $ArithBinaryUnimplemented(src1: Value, src2: Value) returns (dst: Value);
-{{backend.type_requires}} is#Integer(src1) && is#Integer(src2);
-ensures is#Integer(dst);
+procedure {:inline 1} $ArithBinaryUnimplemented(src1: $Value, src2: $Value) returns (dst: $Value);
+{{backend.type_requires}} is#$Integer(src1) && is#$Integer(src2);
+ensures is#$Integer(dst);
 
-procedure {:inline 1} $Lt(src1: Value, src2: Value) returns (dst: Value)
-{{backend.type_requires}} is#Integer(src1) && is#Integer(src2);
+procedure {:inline 1} $Lt(src1: $Value, src2: $Value) returns (dst: $Value)
+{{backend.type_requires}} is#$Integer(src1) && is#$Integer(src2);
 {
-    dst := Boolean(i#Integer(src1) < i#Integer(src2));
+    dst := $Boolean(i#$Integer(src1) < i#$Integer(src2));
 }
 
-procedure {:inline 1} $Gt(src1: Value, src2: Value) returns (dst: Value)
-{{backend.type_requires}} is#Integer(src1) && is#Integer(src2);
+procedure {:inline 1} $Gt(src1: $Value, src2: $Value) returns (dst: $Value)
+{{backend.type_requires}} is#$Integer(src1) && is#$Integer(src2);
 {
-    dst := Boolean(i#Integer(src1) > i#Integer(src2));
+    dst := $Boolean(i#$Integer(src1) > i#$Integer(src2));
 }
 
-procedure {:inline 1} $Le(src1: Value, src2: Value) returns (dst: Value)
-{{backend.type_requires}} is#Integer(src1) && is#Integer(src2);
+procedure {:inline 1} $Le(src1: $Value, src2: $Value) returns (dst: $Value)
+{{backend.type_requires}} is#$Integer(src1) && is#$Integer(src2);
 {
-    dst := Boolean(i#Integer(src1) <= i#Integer(src2));
+    dst := $Boolean(i#$Integer(src1) <= i#$Integer(src2));
 }
 
-procedure {:inline 1} $Ge(src1: Value, src2: Value) returns (dst: Value)
-{{backend.type_requires}} is#Integer(src1) && is#Integer(src2);
+procedure {:inline 1} $Ge(src1: $Value, src2: $Value) returns (dst: $Value)
+{{backend.type_requires}} is#$Integer(src1) && is#$Integer(src2);
 {
-    dst := Boolean(i#Integer(src1) >= i#Integer(src2));
+    dst := $Boolean(i#$Integer(src1) >= i#$Integer(src2));
 }
 
-procedure {:inline 1} $And(src1: Value, src2: Value) returns (dst: Value)
-{{backend.type_requires}} is#Boolean(src1) && is#Boolean(src2);
+procedure {:inline 1} $And(src1: $Value, src2: $Value) returns (dst: $Value)
+{{backend.type_requires}} is#$Boolean(src1) && is#$Boolean(src2);
 {
-    dst := Boolean(b#Boolean(src1) && b#Boolean(src2));
+    dst := $Boolean(b#$Boolean(src1) && b#$Boolean(src2));
 }
 
-procedure {:inline 1} $Or(src1: Value, src2: Value) returns (dst: Value)
-{{backend.type_requires}} is#Boolean(src1) && is#Boolean(src2);
+procedure {:inline 1} $Or(src1: $Value, src2: $Value) returns (dst: $Value)
+{{backend.type_requires}} is#$Boolean(src1) && is#$Boolean(src2);
 {
-    dst := Boolean(b#Boolean(src1) || b#Boolean(src2));
+    dst := $Boolean(b#$Boolean(src1) || b#$Boolean(src2));
 }
 
-procedure {:inline 1} $Not(src: Value) returns (dst: Value)
-{{backend.type_requires}} is#Boolean(src);
+procedure {:inline 1} $Not(src: $Value) returns (dst: $Value)
+{{backend.type_requires}} is#$Boolean(src);
 {
-    dst := Boolean(!b#Boolean(src));
+    dst := $Boolean(!b#$Boolean(src));
 }
 
 // Pack and Unpack are auto-generated for each type T
@@ -839,47 +839,47 @@ procedure {:inline 1} $Not(src: Value) returns (dst: Value)
 // Transaction
 // -----------
 
-type {:datatype} Transaction;
-var $txn: Transaction;
-function {:constructor} Transaction(sender: int) : Transaction;
+type {:datatype} $Transaction;
+var $txn: $Transaction;
+function {:constructor} $Transaction(sender: int) : $Transaction;
 
 
 // ==================================================================================
 // Native Vector Type
 
-function {:inline} $Vector_type_value(tv: TypeValue): TypeValue {
-    VectorType(tv)
+function {:inline} $Vector_type_value(tv: $TypeValue): $TypeValue {
+    $VectorType(tv)
 }
 
-function {:inline} $Vector_is_well_formed(v: Value): bool {
-    is#Vector(v) &&
+function {:inline} $Vector_is_well_formed(v: $Value): bool {
+    is#$Vector(v) &&
     (
-        var va := v#Vector(v);
+        var va := v#$Vector(v);
         (
-            var l := l#ValueArray(va);
+            var l := l#$ValueArray(va);
             0 <= l &&
-            (forall x: int :: {v#ValueArray(va)[x]} x < 0 || x >= l ==> v#ValueArray(va)[x] == DefaultValue())
+            (forall x: int :: {v#$ValueArray(va)[x]} x < 0 || x >= l ==> v#$ValueArray(va)[x] == $DefaultValue())
         )
     )
 }
 
-procedure {:inline 1} $Vector_empty(ta: TypeValue) returns (v: Value) {
+procedure {:inline 1} $Vector_empty(ta: $TypeValue) returns (v: $Value) {
     v := $mk_vector();
 }
 
-procedure {:inline 1} $Vector_is_empty(ta: TypeValue, v: Value) returns (b: Value) {
-    assume is#Vector(v);
-    b := Boolean($vlen(v) == 0);
+procedure {:inline 1} $Vector_is_empty(ta: $TypeValue, v: $Value) returns (b: $Value) {
+    assume is#$Vector(v);
+    b := $Boolean($vlen(v) == 0);
 }
 
-procedure {:inline 1} $Vector_push_back(ta: TypeValue, v: Value, val: Value) returns (v': Value) {
-    assume is#Vector(v);
+procedure {:inline 1} $Vector_push_back(ta: $TypeValue, v: $Value, val: $Value) returns (v': $Value) {
+    assume is#$Vector(v);
     v' := $push_back_vector(v, val);
 }
 
-procedure {:inline 1} $Vector_pop_back(ta: TypeValue, v: Value) returns (e: Value, v': Value) {
+procedure {:inline 1} $Vector_pop_back(ta: $TypeValue, v: $Value) returns (e: $Value, v': $Value) {
     var len: int;
-    assume is#Vector(v);
+    assume is#$Vector(v);
     len := $vlen(v);
     if (len == 0) {
         $abort_flag := true;
@@ -889,28 +889,28 @@ procedure {:inline 1} $Vector_pop_back(ta: TypeValue, v: Value) returns (e: Valu
     v' := $pop_back_vector(v);
 }
 
-procedure {:inline 1} $Vector_append(ta: TypeValue, v: Value, other: Value) returns (v': Value) {
-    assume is#Vector(v);
-    assume is#Vector(other);
+procedure {:inline 1} $Vector_append(ta: $TypeValue, v: $Value, other: $Value) returns (v': $Value) {
+    assume is#$Vector(v);
+    assume is#$Vector(other);
     v' := $append_vector(v, other);
 }
 
-procedure {:inline 1} $Vector_reverse(ta: TypeValue, v: Value) returns (v': Value) {
-    assume is#Vector(v);
+procedure {:inline 1} $Vector_reverse(ta: $TypeValue, v: $Value) returns (v': $Value) {
+    assume is#$Vector(v);
     v' := $reverse_vector(v);
 }
 
-procedure {:inline 1} $Vector_length(ta: TypeValue, v: Value) returns (l: Value) {
-    assume is#Vector(v);
-    l := Integer($vlen(v));
+procedure {:inline 1} $Vector_length(ta: $TypeValue, v: $Value) returns (l: $Value) {
+    assume is#$Vector(v);
+    l := $Integer($vlen(v));
 }
 
-procedure {:inline 1} $Vector_borrow(ta: TypeValue, src: Value, i: Value) returns (dst: Value) {
+procedure {:inline 1} $Vector_borrow(ta: $TypeValue, src: $Value, i: $Value) returns (dst: $Value) {
     var i_ind: int;
 
-    assume is#Vector(src);
-    assume is#Integer(i);
-    i_ind := i#Integer(i);
+    assume is#$Vector(src);
+    assume is#$Integer(i);
+    i_ind := i#$Integer(i);
     if (i_ind < 0 || i_ind >= $vlen(src)) {
         $abort_flag := true;
         return;
@@ -918,35 +918,35 @@ procedure {:inline 1} $Vector_borrow(ta: TypeValue, src: Value, i: Value) return
     dst := $vmap(src)[i_ind];
 }
 
-procedure {:inline 1} $Vector_borrow_mut(ta: TypeValue, v: Value, index: Value) returns (dst: Reference, v': Value)
-{{backend.type_requires}} is#Integer(index);
+procedure {:inline 1} $Vector_borrow_mut(ta: $TypeValue, v: $Value, index: $Value) returns (dst: $Reference, v': $Value)
+{{backend.type_requires}} is#$Integer(index);
 {
     var i_ind: int;
 
-    i_ind := i#Integer(index);
-    assume is#Vector(v);
+    i_ind := i#$Integer(index);
+    assume is#$Vector(v);
     if (i_ind < 0 || i_ind >= $vlen(v)) {
         $abort_flag := true;
         return;
     }
-    dst := Reference(Local(0), Path(p#Path(EmptyPath)[0 := i_ind], 1), $vmap(v)[i_ind]);
+    dst := $Reference($Local(0), $Path(p#$Path($EmptyPath)[0 := i_ind], 1), $vmap(v)[i_ind]);
     v' := v;
 }
 
-procedure {:inline 1} $Vector_destroy_empty(ta: TypeValue, v: Value) {
+procedure {:inline 1} $Vector_destroy_empty(ta: $TypeValue, v: $Value) {
     if ($vlen(v) != 0) {
       $abort_flag := true;
     }
 }
 
-procedure {:inline 1} $Vector_swap(ta: TypeValue, v: Value, i: Value, j: Value) returns (v': Value)
-{{backend.type_requires}} is#Integer(i) && is#Integer(j);
+procedure {:inline 1} $Vector_swap(ta: $TypeValue, v: $Value, i: $Value, j: $Value) returns (v': $Value)
+{{backend.type_requires}} is#$Integer(i) && is#$Integer(j);
 {
     var i_ind: int;
     var j_ind: int;
-    assume is#Vector(v);
-    i_ind := i#Integer(i);
-    j_ind := i#Integer(j);
+    assume is#$Vector(v);
+    i_ind := i#$Integer(i);
+    j_ind := i#$Integer(j);
     if (i_ind >= $vlen(v) || j_ind >= $vlen(v) || i_ind < 0 || j_ind < 0) {
         $abort_flag := true;
         return;
@@ -954,13 +954,13 @@ procedure {:inline 1} $Vector_swap(ta: TypeValue, v: Value, i: Value, j: Value) 
     v' := $swap_vector(v, i_ind, j_ind);
 }
 
-procedure {:inline 1} $Vector_remove(ta: TypeValue, v: Value, i: Value) returns (e: Value, v': Value)
-{{backend.type_requires}} is#Integer(i);
+procedure {:inline 1} $Vector_remove(ta: $TypeValue, v: $Value, i: $Value) returns (e: $Value, v': $Value)
+{{backend.type_requires}} is#$Integer(i);
 {
     var i_ind: int;
 
-    assume is#Vector(v);
-    i_ind := i#Integer(i);
+    assume is#$Vector(v);
+    i_ind := i#$Integer(i);
     if (i_ind < 0 || i_ind >= $vlen(v)) {
         $abort_flag := true;
         return;
@@ -969,14 +969,14 @@ procedure {:inline 1} $Vector_remove(ta: TypeValue, v: Value, i: Value) returns 
     v' := $remove_vector(v, i_ind);
 }
 
-procedure {:inline 1} $Vector_swap_remove(ta: TypeValue, v: Value, i: Value) returns (e: Value, v': Value)
-{{backend.type_requires}} is#Integer(i);
+procedure {:inline 1} $Vector_swap_remove(ta: $TypeValue, v: $Value, i: $Value) returns (e: $Value, v': $Value)
+{{backend.type_requires}} is#$Integer(i);
 {
     var i_ind: int;
     var len: int;
 
-    assume is#Vector(v);
-    i_ind := i#Integer(i);
+    assume is#$Vector(v);
+    i_ind := i#$Integer(i);
     len := $vlen(v);
     if (i_ind < 0 || i_ind >= len) {
         $abort_flag := true;
@@ -986,41 +986,41 @@ procedure {:inline 1} $Vector_swap_remove(ta: TypeValue, v: Value, i: Value) ret
     v' := $pop_back_vector($swap_vector(v, i_ind, len-1));
 }
 
-procedure {:inline 1} $Vector_contains(ta: TypeValue, v: Value, e: Value) returns (res: Value)  {
-    assume is#Vector(v);
-    res := Boolean($contains_vector(v, e));
+procedure {:inline 1} $Vector_contains(ta: $TypeValue, v: $Value, e: $Value) returns (res: $Value)  {
+    assume is#$Vector(v);
+    res := $Boolean($contains_vector(v, e));
 }
 
 // FIXME: This procedure sometimes (not always) make the test (performance_200511) very slow (> 10 mins) or hang
 // although this is not used in the test script (performance_200511). The test finishes in 20 secs when it works fine.
-procedure {:inline 1} $Vector_index_of(ta: TypeValue, v: Value, e: Value) returns (res1: Value, res2: Value);
-requires is#Vector(v);
-ensures is#Boolean(res1);
-ensures is#Integer(res2);
-ensures 0 <= i#Integer(res2) && i#Integer(res2) < $vlen(v);
-ensures res1 == Boolean($contains_vector(v, e));
-ensures b#Boolean(res1) ==> IsEqual($vmap(v)[i#Integer(res2)], e);
-ensures b#Boolean(res1) ==> (forall i:int :: 0<=i && i<i#Integer(res2) ==> !IsEqual($vmap(v)[i], e));
-ensures !b#Boolean(res1) ==> i#Integer(res2) == 0;
+procedure {:inline 1} $Vector_index_of(ta: $TypeValue, v: $Value, e: $Value) returns (res1: $Value, res2: $Value);
+requires is#$Vector(v);
+ensures is#$Boolean(res1);
+ensures is#$Integer(res2);
+ensures 0 <= i#$Integer(res2) && i#$Integer(res2) < $vlen(v);
+ensures res1 == $Boolean($contains_vector(v, e));
+ensures b#$Boolean(res1) ==> $IsEqual($vmap(v)[i#$Integer(res2)], e);
+ensures b#$Boolean(res1) ==> (forall i:int :: 0<=i && i<i#$Integer(res2) ==> !$IsEqual($vmap(v)[i], e));
+ensures !b#$Boolean(res1) ==> i#$Integer(res2) == 0;
 
 // FIXME: This alternative definition has the same issue as the other one above.
 // TODO: Delete this when unnecessary
-//procedure {:inline 1} $Vector_index_of(ta: TypeValue, v: Value, e: Value) returns (res1: Value, res2: Value) {
+//procedure {:inline 1} $Vector_index_of(ta: $TypeValue, v: $Value, e: $Value) returns (res1: $Value, res2: $Value) {
 //    var b: bool;
 //    var i: int;
-//    assume is#Vector(v);
+//    assume is#$Vector(v);
 //    b := $contains_vector(v, e);
 //    if (b) {
 //        havoc i;
 //        assume 0 <= i && i < $vlen(v);
-//        assume IsEqual($vmap(v)[i], e);
-//        assume (forall j:int :: 0<=j && j<i ==> !IsEqual($vmap(v)[j], e));
+//        assume $IsEqual($vmap(v)[i], e);
+//        assume (forall j:int :: 0<=j && j<i ==> !$IsEqual($vmap(v)[j], e));
 //    }
 //    else {
 //        i := 0;
 //    }
-//    res1 := Boolean(b);
-//    res2 := Integer(i);
+//    res1 := $Boolean(b);
+//    res2 := $Integer(i);
 //}
 
 // ==================================================================================
@@ -1032,50 +1032,50 @@ ensures !b#Boolean(res1) ==> i#Integer(res2) == 0;
 // common to assume in code there are no hash collisions in practice.  Fortunately,
 // Boogie is not smart enough to recognized that there is an inconsistency.
 // FIXME: If we were using a reliable extensional theory of arrays, and if we could use ==
-// instead of IsEqual, we might be able to avoid so many quantified formulas by
+// instead of $IsEqual, we might be able to avoid so many quantified formulas by
 // using a sha2_inverse function in the ensures conditions of Hash_sha2_256 to
 // assert that sha2/3 are injections without using global quantified axioms.
 
 
-function {:inline} $Hash_sha2($m: Memory, $txn: Transaction, val: Value): Value {
+function {:inline} $Hash_sha2($m: $Memory, $txn: $Transaction, val: $Value): $Value {
     $Hash_sha2_core(val)
 }
 
-function $Hash_sha2_core(val: Value): Value;
+function $Hash_sha2_core(val: $Value): $Value;
 
 // This says that Hash_sha2 respects isEquals (this would be automatic if we had an
 // extensional theory of arrays and used ==, which has the substitution property
 // for functions).
-axiom (forall v1,v2: Value :: $Vector_is_well_formed(v1) && $Vector_is_well_formed(v2)
-       && IsEqual(v1, v2) ==> IsEqual($Hash_sha2_core(v1), $Hash_sha2_core(v2)));
+axiom (forall v1,v2: $Value :: $Vector_is_well_formed(v1) && $Vector_is_well_formed(v2)
+       && $IsEqual(v1, v2) ==> $IsEqual($Hash_sha2_core(v1), $Hash_sha2_core(v2)));
 
 // This says that Hash_sha2 is an injection
-axiom (forall v1,v2: Value :: $Vector_is_well_formed(v1) && $Vector_is_well_formed(v2)
-        && IsEqual($Hash_sha2_core(v1), $Hash_sha2_core(v2)) ==> IsEqual(v1, v2));
+axiom (forall v1,v2: $Value :: $Vector_is_well_formed(v1) && $Vector_is_well_formed(v2)
+        && $IsEqual($Hash_sha2_core(v1), $Hash_sha2_core(v2)) ==> $IsEqual(v1, v2));
 
 // This procedure has no body. We want Boogie to just use its requires
 // and ensures properties when verifying code that calls it.
-procedure $Hash_sha2_256(val: Value) returns (res: Value);
+procedure $Hash_sha2_256(val: $Value) returns (res: $Value);
 // It will still work without this, but this helps verifier find more reasonable counterexamples.
 {{backend.type_requires}} $IsValidU8Vector(val);
-ensures res == $Hash_sha2_core(val);     // returns Hash_sha2 value
+ensures res == $Hash_sha2_core(val);     // returns Hash_sha2 Value
 ensures $IsValidU8Vector(res);    // result is a legal vector of U8s.
 ensures $vlen(res) == 32;               // result is 32 bytes.
 
 // similarly for Hash_sha3
-function {:inline} $Hash_sha3($m: Memory, $txn: Transaction, val: Value): Value {
+function {:inline} $Hash_sha3($m: $Memory, $txn: $Transaction, val: $Value): $Value {
     $Hash_sha3_core(val)
 }
-function $Hash_sha3_core(val: Value): Value;
+function $Hash_sha3_core(val: $Value): $Value;
 
-axiom (forall v1,v2: Value :: $Vector_is_well_formed(v1) && $Vector_is_well_formed(v2)
-       && IsEqual(v1, v2) ==> IsEqual($Hash_sha3_core(v1), $Hash_sha3_core(v2)));
+axiom (forall v1,v2: $Value :: $Vector_is_well_formed(v1) && $Vector_is_well_formed(v2)
+       && $IsEqual(v1, v2) ==> $IsEqual($Hash_sha3_core(v1), $Hash_sha3_core(v2)));
 
-axiom (forall v1,v2: Value :: $Vector_is_well_formed(v1) && $Vector_is_well_formed(v2)
-        && IsEqual($Hash_sha3_core(v1), $Hash_sha3_core(v2)) ==> IsEqual(v1, v2));
+axiom (forall v1,v2: $Value :: $Vector_is_well_formed(v1) && $Vector_is_well_formed(v2)
+        && $IsEqual($Hash_sha3_core(v1), $Hash_sha3_core(v2)) ==> $IsEqual(v1, v2));
 
-procedure $Hash_sha3_256(val: Value) returns (res: Value);
-ensures res == $Hash_sha3_core(val);     // returns Hash_sha3 value
+procedure $Hash_sha3_256(val: $Value) returns (res: $Value);
+ensures res == $Hash_sha3_core(val);     // returns Hash_sha3 Value
 ensures $IsValidU8Vector(res);    // result is a legal vector of U8s.
 ensures $vlen(res) == 32;               // result is 32 bytes.
 
@@ -1085,14 +1085,14 @@ ensures $vlen(res) == 32;               // result is 32 bytes.
 // TODO: this function clashes with a similar version in older libraries. This is solved by a hack where the
 // translator appends _OLD to the name when encountering this. The hack shall be removed once old library
 // sources are not longer used.
-procedure {:inline 1} $LibraAccount_save_account_OLD(ta: TypeValue, balance: Value, account: Value, addr: Value) {
+procedure {:inline 1} $LibraAccount_save_account_OLD(ta: $TypeValue, balance: $Value, account: $Value, addr: $Value) {
     var a: int;
-    var t_T: TypeValue;
-    var l_T: Location;
-    var t_Balance: TypeValue;
-    var l_Balance: Location;
+    var t_T: $TypeValue;
+    var l_T: $Location;
+    var t_Balance: $TypeValue;
+    var l_Balance: $Location;
 
-    a := a#Address(addr);
+    a := a#$Address(addr);
     t_T := $LibraAccount_T_type_value();
     if ($ResourceExistsRaw($m, t_T, a)) {
         $abort_flag := true;
@@ -1105,45 +1105,45 @@ procedure {:inline 1} $LibraAccount_save_account_OLD(ta: TypeValue, balance: Val
         return;
     }
 
-    l_T := Global(t_T, a);
-    l_Balance := Global(t_Balance, a);
-    $m := Memory(domain#Memory($m)[l_T := true][l_Balance := true], contents#Memory($m)[l_T := account][l_Balance := balance]);
+    l_T := $Global(t_T, a);
+    l_Balance := $Global(t_Balance, a);
+    $m := $Memory(domain#$Memory($m)[l_T := true][l_Balance := true], contents#$Memory($m)[l_T := account][l_Balance := balance]);
 }
 
 procedure {:inline 1} $LibraAccount_save_account(
-       t_Token: TypeValue, t_AT: TypeValue, account_type: Value, balance: Value,
-       account: Value, event_generator: Value, addr: Value) {
+       t_Token: $TypeValue, t_AT: $TypeValue, account_type: $Value, balance: $Value,
+       account: $Value, event_generator: $Value, addr: $Value) {
     // TODO: implement this
     assert false;
 }
 
 procedure {:inline 1} $LibraAccount_create_signer(
-  addr: Value
-) returns (signer: Value) {
+  addr: $Value
+) returns (signer: $Value) {
     // A signer is currently identical to an address.
     signer := addr;
 }
 
 procedure {:inline 1} $LibraAccount_destroy_signer(
-  signer: Value
+  signer: $Value
 ) {
   return;
 }
 
-procedure {:inline 1} $LibraAccount_write_to_event_store(ta: TypeValue, guid: Value, count: Value, msg: Value) {
+procedure {:inline 1} $LibraAccount_write_to_event_store(ta: $TypeValue, guid: $Value, count: $Value, msg: $Value) {
     // TODO: this is used in old library sources, remove it once those sources are not longer used in tests.
     // This function is modeled as a no-op because the actual side effect of this native function is not observable from the Move side.
 }
 
-procedure {:inline 1} $Event_write_to_event_store(ta: TypeValue, guid: Value, count: Value, msg: Value) {
+procedure {:inline 1} $Event_write_to_event_store(ta: $TypeValue, guid: $Value, count: $Value, msg: $Value) {
     // This function is modeled as a no-op because the actual side effect of this native function is not observable from the Move side.
 }
 
 // ==================================================================================
 // Native signer
 
-procedure {:inline 1} $Signer_borrow_address(signer: Value) returns (res: Value)
-    {{backend.type_requires}} is#Address(signer);
+procedure {:inline 1} $Signer_borrow_address(signer: $Value) returns (res: $Value)
+    {{backend.type_requires}} is#$Address(signer);
 {
     res := signer;
 }
@@ -1154,15 +1154,15 @@ procedure {:inline 1} $Signer_borrow_address(signer: Value) returns (res: Value)
 
 // TODO: implement the below methods
 
-procedure {:inline 1} $Signature_ed25519_validate_pubkey(public_key: Value) returns (res: Value) {
+procedure {:inline 1} $Signature_ed25519_validate_pubkey(public_key: $Value) returns (res: $Value) {
     assert false; // $Signature_ed25519_validate_pubkey not implemented
 }
 
-procedure {:inline 1} $Signature_ed25519_verify(signature: Value, public_key: Value, message: Value) returns (res: Value) {
+procedure {:inline 1} $Signature_ed25519_verify(signature: $Value, public_key: $Value, message: $Value) returns (res: $Value) {
     assert false; // $Signature_ed25519_verify not implemented
 }
 
-procedure {:inline 1} Signature_ed25519_threshold_verify(bitmap: Value, signature: Value, public_key: Value, message: Value) returns (res: Value) {
+procedure {:inline 1} Signature_ed25519_threshold_verify(bitmap: $Value, signature: $Value, public_key: $Value, message: $Value) returns (res: $Value) {
     assert false; // Signature_ed25519_threshold_verify not implemented
 }
 
@@ -1174,32 +1174,32 @@ procedure {:inline 1} Signature_ed25519_threshold_verify(bitmap: Value, signatur
 // Serialize is modeled as an uninterpreted function, with an additional
 // axiom to say it's an injection.
 
-function {:inline} $LCS_serialize($m: Memory, $txn: Transaction, ta: TypeValue, v: Value): Value {
+function {:inline} $LCS_serialize($m: $Memory, $txn: $Transaction, ta: $TypeValue, v: $Value): $Value {
     $LCS_serialize_core(v)
 }
 
-function $LCS_serialize_core(v: Value): Value;
-function $LCS_serialize_core_inv(v: Value): Value;
+function $LCS_serialize_core(v: $Value): $Value;
+function $LCS_serialize_core_inv(v: $Value): $Value;
 // Needed only because IsEqual(v1, v2) is weaker than v1 == v2 in case there is a vector nested inside v1 or v2.
-axiom (forall v1, v2: Value :: IsEqual(v1, v2) ==> $LCS_serialize_core(v1) == $LCS_serialize_core(v2));
+axiom (forall v1, v2: $Value :: $IsEqual(v1, v2) ==> $LCS_serialize_core(v1) == $LCS_serialize_core(v2));
 // Injectivity
-axiom (forall v: Value :: $LCS_serialize_core_inv($LCS_serialize_core(v)) == v);
+axiom (forall v: $Value :: $LCS_serialize_core_inv($LCS_serialize_core(v)) == v);
 
 // This says that serialize returns a non-empty vec<u8>
 {{#if (eq backend.serialize_bound 0)}}
-axiom (forall v: Value :: ( var r := $LCS_serialize_core(v); $IsValidU8Vector(r) && $vlen(r) > 0 ));
+axiom (forall v: $Value :: ( var r := $LCS_serialize_core(v); $IsValidU8Vector(r) && $vlen(r) > 0 ));
 {{else}}
-axiom (forall v: Value :: ( var r := $LCS_serialize_core(v); $IsValidU8Vector(r) && $vlen(r) > 0 &&
+axiom (forall v: $Value :: ( var r := $LCS_serialize_core(v); $IsValidU8Vector(r) && $vlen(r) > 0 &&
                             $vlen(r) <= {{backend.serialize_bound}} ));
 {{/if}}
 
-procedure $LCS_to_bytes(ta: TypeValue, v: Value) returns (res: Value);
+procedure $LCS_to_bytes(ta: $TypeValue, v: $Value) returns (res: $Value);
 ensures res == $LCS_serialize($m, $txn, ta, v);
 ensures $IsValidU8Vector(res);    // result is a legal vector of U8s.
 
 // ==================================================================================
 // Native Signer::get_address
-function $Signer_get_address($m: Memory, $txn: Transaction, signer: Value): Value
+function $Signer_get_address($m: $Memory, $txn: $Transaction, signer: $Value): $Value
 {
     // A signer is currently identical to an address.
     signer
